bound-utils.lisp
@@ -1,0 +1,49 @@
+
+
+;; bound will make any input integer p to be within interval [0, N)
+(defun bound (p N)
+  (declare (xargs :guard (and (integerp p)
+                              (integerp N))))
+  (if (< N 0)
+      -1
+    (if (< p 0)
+        0
+      (if (< p N)
+          p
+        (- N 1)))))
+
+(defthm bound-type-ok (implies (and (integer-listp l)
+                                    (consp l)
+                                    (integerp x))
+                               (integerp (nth (bound x (length l)) l))))
+
+(defthm bound-ok (implies (and (< 0 N)
+                               (integerp N)
+                               (integerp x))
+                          (and (integerp (bound x N))
+                               (< (bound x N) N))))
+
+(DEFTHM MEMBER-IF-BOUNDED
+        (IMPLIES (AND (INTEGER-LISTP L)
+                      (CONSP L)
+                      (INTEGERP X)
+                      (< X (LENGTH L)))
+                 (MEMBER (NTH X L) L)))
+
+(defthm bound-mem-ok (implies (and (integer-listp l)
+                                   (consp l)
+                                   (integerp x))
+                              (member (nth (bound x (length l)) l) l)))
+
+(defthm bound-mem-int (implies (and (integer-listp l)
+                                    (consp l)
+                                    (integerp x))
+                               (integerp (nth (bound x (length l)) l))))
+
+(defthm update-nth-buf-ok
+    (implies (and (bufferp buf)
+                  (integerp n1)
+                  (integerp n2)
+                  (<= 0 n1)
+                  (< n1 (length buf)))
+             (bufferp (update-nth n1 n2 buf))))
